# Problem Statement

![](!imgdir/e537244a52fc535fbf6b6cf525bd2ff1f2ddba83.png)

# Solution

## Goal

Compute the solution to the given equation and parameters, as well as the closed form solution.

## Given

The following equation of motion is given:

$$
\ddot{x}+2 \dot{x}+2 x=0
$$

as well as the following parameters:

!EQDefine(x_0)(x0)(0)(!_mm)
!EQDefine(v_0)(v0)(1)(!_mmps)

$$
\begin{aligned}
    !AGiven(x0)\\
    !AGiven(v0)
\end{aligned}
$$

## Working

<!-- SOS -->

We know that:

$$
\zeta=\frac{c}{c_{c r}}=\frac{c}{2 m \omega_{n}}=\frac{c}{2 \sqrt{k m}}
$$

and that:

$$
\omega_{d}=\omega_{n} \sqrt{1-\zeta^{2}}
$$

Given the equation of motion, we know:

!EQDefine(m)(m)(1)()
!EQDefine(c)(c)(2)()
!EQDefine(k)(k)(2)()

$$
\begin{aligned}
    !AGiven(m)\\
    !AGiven(c)\\
    !AGiven(k)
\end{aligned}
$$

First, we must determine the damping ratio:

!define(ratio)(!math(!c/(2*(!k*!m)^0.5)))

$$
\begin{aligned}
    \zeta &= \frac{!c_v}{2\sqrt{!k_v\cdot!m_v}}\\
    &= \frac{1}{\sqrt{2}}\\
    \zeta &= !mathr(!ratio)(4)
\end{aligned}
$$

As $\zeta < 1$, the system is underdamped.
For such a system, the equation of motion is given (pgs. 25-26) by:

$$
x(t)=A e^{-\zeta \omega_{n} t} \sin \left(\omega_{d} t+\phi\right)
$$

as well as the following:

$$
A=\sqrt{\frac{\left(v_{0}+\zeta \omega_{n} x_{0}\right)^{2}+\left(x_{0} \omega_{d}\right)^{2}}{\omega_{d}^{2}}}, \quad \phi=\tan ^{-1} \frac{x_{0} \omega_{d}}{v_{0}+\zeta \omega_{n} x_{0}}
$$

Because $!x0_f=0$, we can simplify rapidly:

$$
\begin{aligned}
    A&=\sqrt{\frac{\left(\cancelto{0}{\zeta \omega_{n} x_{0}} + v_{0}\right)^{2}+\cancelto{0}{\left(x_{0} \omega_{d}\right)^{2}}}{\omega_{d}^{2}}}\\
    &=\sqrt{\frac{v_{0}^{2}}{\omega_{d}^{2}}}\\
    A&=\frac{v_{0}}{\omega_{d}}\\
\end{aligned}
$$

$$
\begin{aligned}
    \phi &= \tan ^{-1} \cancelto{0}{\frac{x_{0} \omega_{d}}{v_{0}+\zeta \omega_{n} x_{0}}}\\
    \phi &= 0
\end{aligned}
$$

We know that:

$$
c_{c r}=2 m \omega_{n}=2 \sqrt{k m}
$$

thus:

!define(wn)(!math((!k/!m)^0.5))

$$
\begin{aligned}
    \omega_{n}&=\sqrt{\frac{k}{m}}\\ 
    &= \sqrt{2}
\end{aligned}
$$

and so:

$$
\begin{aligned}
    \omega_d &= \sqrt{\frac{k}{m}} \sqrt{1-\zeta^2}
\end{aligned}
$$

Substituting into amplitude $A$, along with real values:

!define(A)(!math(1/(((2)^0.5)*((1-!ratio)^0.5))))

$$
\begin{aligned}
    A&=\frac{v_{0}}{\sqrt{\frac{k}{m}} \sqrt{1-\zeta^2}}\\
\end{aligned}
$$

Moving back to our equation of motion, we may substitute known values in to find our final answer:

$$
\begin{aligned}
    x(t)&=A e^{-\zeta \omega_{n} t} \sin \left(\omega_{d} t+\phi\right)\\
    &=\frac{!v0_v}{\sqrt{\frac{!k_v}{!m_v}} \sqrt{1-\frac{1}{\sqrt{2}}^2}} e^{-t} \sin \left(\sqrt{\frac{!k_v}{!m_v}} \sqrt{1-\frac{1}{\sqrt{2}}^2} t\right)\\
    &= \frac{1}{\sqrt{2}\sqrt{\frac{1}{2}}}e^{-t}\sin{\left( \sqrt{2}\sqrt{\frac{1}{2}} t \right)}\\
    !Answer(x(t))(=)(e^{-t} \sin{t} !_mm)
\end{aligned}
$$