# Problem Statement

![](!imgdir/screenshot_PP9HT68FdaAFeyGe.png)

# Solution

## Goal

Determine the equations of motion and calculate $\omega_n$ and $\omega_d$.

## Known

Spring is massless.

!EQDefine(\zeta)(z)(0.01)()

$$
\begin{aligned}
    !AGiven(z)
\end{aligned}
$$

## Working

<!-- SOS -->

We know (pg. 32):

$$
\sum_{i} M_{0 i}=J \ddot{\theta} = J \alpha
$$

We also know mass moment of inertia of a point mass is given by:

$$
J=m l^{2}
$$

as such, our total mass moment of inertia is summed to be:

$$
J_{\text{total}} = J + m l^2
$$

We may then equate these to the sum of moments produced by forces. First, we know the damping force due to the oil is given by (pg. 22):

$$
f_{c}=c \dot{x}(t)
$$

where the force $f_c$ opposes the motion $\dot{x}$. 
The force due to the spring is known to be:

$$
F = kx
$$

where the force $F$ opposes the displacement.
We know a moment to be $M=Fl$, so we can equate as planned earlier:

$$
\left( J + m l^2 \right) \ddot{\theta} = - \left( kx + c \dot{x} \right) l
$$

the displacement $x$ may be found using $\theta$:

$$
x = l\sin{\left( \theta \right)}
$$

however, for small angles , we may approximate $\theta\approx \sin{\left( \theta \right)}$, thus:

$$
x = l\theta
$$

Hence:

$$
\begin{aligned}
    \left( J + m l^2 \right) \ddot{\theta} &= - \left( k l \theta + c l \dot{\theta} \right) l\\
    \left( J + m l^2 \right) \ddot{\theta} + \left( k l\theta + c l \dot{\theta} \right) l &= 0\\
    \left( J + m l^2 \right) \ddot{\theta} + c l^2 \dot{\theta} + k l^2 \theta  &= 0\\
    \ddot{\theta} + \frac{c l^2 \dot{\theta}}{ J + m l^2} + \frac{k l^2 \theta }{J + m l^2} &= 0\\
    \ddot{\theta} + \dot{\theta} \left( \frac{c l^2}{ J + m l^2} \right) + \theta \left( \frac{k l^2 }{J + m l^2} \right) &= 0\\
\end{aligned}
$$

Using a known relationship, we know that the undamped natural frequency is found to be:

$$
\begin{aligned}
    !Answer(\omega_n)(=)(\sqrt{\frac{k l^2 }{J + m l^2}} !_rads)
\end{aligned}
$$

we also know $\omega_d$, which we may solve for:

$$
\begin{aligned}
    \omega_{d} &= \omega_{n} \sqrt{1-\zeta^{2}}\\
    &= \sqrt{\frac{k l^2 }{J + m l^2}} \sqrt{1-!z_v^2}\\
    !Answer(\omega_d)(=)(!mathr((1-!z^2)^0.5)(6)\sqrt{\frac{k l^2 }{J + m l^2}} !_rads)\\
\end{aligned}
$$