# Problem Statement

![](!imgdir/screenshot_58mmZSNBnjdfGlgX.png)

# Solution

## Goal

## Working

<!-- SOS -->

We may define the mass of the bar to be $m_B$.

The height of the tip may be calculated as follows:

$$
h_T = l \left( 1 - \cos{\theta} \right)
$$

similarly, the height of the midpoint of the bar:

$$
h_B = \frac{l}{2} \left( 1 - \cos{\theta} \right)
$$

Potential energy is calculated by using:

$$
\text{PE} = U = mgh
$$

As such, the total potential energy of the system is given by:

$$
\begin{aligned}
    U &= g\left( m_T\cdot h_T + m_B \cdot h_B \right)\\
    &= g\left( m_T\cdot l \left( 1 - \cos{\theta} \right) + m_B \cdot \frac{l}{2} \left( 1 - \cos{\theta} \right) \right)\\
    &= gl\left(1-\cos{\theta}\right)\left( m_T + \frac{m_B}{2} \right)\\
\end{aligned}
$$

Kinetic energy for a rigid body is calculated by using:

$$
\text{KE} = T = \frac{1}{2}mv^2 + \frac{1}{2} I_G \omega^2
$$

where $I$ for the point mass is found using:

$$
I = md^2
$$

and for the rod:

$$
I = \frac{1}{3} m l^2
$$

For the two masses, we then say:

$$
I = m_T\cdot l^2 + m_B \cdot \frac{1}{3} l^2
$$

Assuming no friction, kinetic energy plus potential energy is constant:

$$
\begin{aligned}
    \cancel{\frac{1}{2}mv^2} + \frac{1}{2} I_G \omega^2 + gl\left(1-\cos{\theta}\right)\left( m_T + \frac{m_B}{2} \right) &= C\\
    \frac{1}{2} \left( m_T\cdot l^2 + m_B \cdot \frac{1}{3} l^2 \right) \omega^2 + gl\left(1-\cos{\theta}\right)\left( m_T + \frac{m_B}{2} \right) &= C\\
    \frac{l}{2} \left( m_T + m_B \cdot \frac{1}{3} \right) \dot{\theta}^2 + g\left(1-\cos{\theta}\right)\left( m_T + \frac{m_B}{2} \right) &= C\\
\end{aligned}
$$

taking the derivative with respect to time:

$$
\begin{aligned}
    l \left( m_T + m_B \cdot \frac{1}{3} \right) \dot{\theta} \ddot{\theta} + g\left(\sin{\theta}\right)\left( m_T + \frac{m_B}{2} \right)\dot{\theta} &= 0\\
    l \left( m_T + m_B \cdot \frac{1}{3} \right) \ddot{\theta} + g\left(\sin{\theta}\right)\left( m_T + \frac{m_B}{2} \right) &= 0\\
\end{aligned}
$$

we may approximate $\sin{\theta}\approx\theta$ for small angles, and so rearrange to match known format:

$$
\begin{aligned}
    l \left( m_T + m_B \cdot \frac{1}{3} \right) \ddot{\theta} + g \theta \left( m_T + \frac{m_B}{2} \right) &= 0\\
    \ddot{\theta} + \theta \frac{g \left( m_T + \frac{m_B}{2} \right)}{l \left( m_T + m_B \cdot \frac{1}{3} \right)} &= 0\\
    \ddot{\theta} + \theta \frac{g \left( 6m_T + 3m_B \right)}{l \left( 6m_T + 2m_B \right)} &= 0\\
    \ddot{\theta} + \theta \left( \frac{g}{l} \right) \left( \frac{6m_T + 3m_B }{6m_T + 2m_B} \right) &= 0\\
\end{aligned}
$$

knowing this format, we can say:

$$
\begin{aligned}
    !Answer(\omega_n)(=)(\sqrt{\left( \frac{g}{l} \right) \left( \frac{6m_T + 3m_B }{6m_T + 2m_B} \right)})
\end{aligned}
$$