# Problem Statement

![](!imgdir/screenshot_vNNZtwb4wuPqd6uX.png)

# Solution

## Working

<!-- SOS -->

From kinematics:

$$
\begin{aligned}
&x=r \theta \\
&\dot{x}=r \dot{\theta}
\end{aligned}
$$

Kinetic Energy:

$$
\begin{aligned}
\text{From rotation: } &T_{r}=\frac{1}{2} J \dot{\theta}^{2} \\
\text{From linear: } &T_{l}=\frac{1}{2} m \dot{x}^{2}
\end{aligned}
$$

$$
T_{\text{Total}}=\frac{1}{2} J \dot{\theta}^{2}+\frac{1}{2} m \dot{x}^{2}
$$

Potential Energy:

$$
\begin{aligned}
\text{From rotation: } &U_{r}=\frac{1}{2} k_{1} \theta^{2} \\
\text{From linear: } &U_{l}=\frac{1}{2} k_{z} x^{2}
\end{aligned}
$$

$$
U_{\text{Total}}=\frac{1}{2} k_{1} \theta^{2}+\frac{1}{2}k_2 x^2
$$

$$
T+U=\frac{1}{2} J \dot{\theta}^{2}+\frac{1}{2} m \dot{x}^{2}+\frac{1}{2} k_{1} \theta^{2}+\frac{1}{2} k_{2} x^{2}
$$

Substitute $\theta=\frac{x}{r}$

$$
T+U=\frac{1}{2} J\left(\frac{\dot{x}}{r}\right)^{2}+\frac{1}{2} m \dot{x}^{2}+\frac{1}{2} k_{1}\left(\frac{x}{r}\right)^{2}+\frac{1}{2} k_{2} x^{2}
$$

$$
\frac{d(T+U)}{d t}=0 \Rightarrow \frac{J \ddot{x} \dot{x}}{r^{2}}+m \ddot{x} \dot{x}+\frac{k_{1}}{r^{2}} x \dot{x}+k_{2} x \dot{x}=0
$$

$$
\frac{1}{\cancel{\dot{x}}}\left[\frac{j \ddot{x} \cancel{\dot{x}}}{r^{2}}+m \ddot{x} \cancel{\dot{x}}+\frac{k_{1}}{r^{2}} x \cancel{\dot{x}}+k_{2} x \cancel{\dot{x}}=0\right]
$$

$$
\boxed{\left(\frac{J}{r^{2}}+m\right) \ddot{x}+\left(\frac{k_{1}}{r^{2}}+k_{2}\right) x=0}
$$

$$
\omega_{n}=\sqrt{\frac{k_{1}+r^{2} k_{2}}{J+m r^{2}}}
$$