# Problem Statement

![](!imgdir/screenshot_DU88TXbUUXp3bgNf.png)

# Solution

<!-- SOS -->

Let $\theta=0$ be the point of lowest potential energy.

$$
\begin{aligned}
    x_{k} &= l_{1} \theta
    x_{m}&=l_{2} \theta
    h&=(1-\cos \theta) l_{2}
\end{aligned}
$$

$$
\begin{aligned}
    \text{Kinetic energy: } T&=\frac{1}{2} m \dot{x}_{m}^{2}=\frac{1}{2} m\left(l_{2} \dot{\theta}\right)^{2}\\
    \text{Potential energy: } U&=\frac{1}{2} k x_{k}^{2}+m g h\\
    U&=\frac{1}{2} k\left(l_{1} \theta\right)^{2}+m g(1-\cos \theta) l_{2}
\end{aligned}
$$

$$
T+U=\frac{1}{2} m l_{2}^{2} \dot{\theta}^{2}+\frac{1}{2} k l_{1}^{2} \theta^{2}+m g l_{2}-m g l_{2} \cos \theta
$$

$$
\frac{d}{d t}(T+U)=m l_{2}^{2} \dot{\theta} \ddot{\theta}+k l_{1}^{2} \theta \dot{\theta}+m g l_{2}(\sin \theta) \dot{\theta}=0
$$

We may approximate $\theta=\sin{\theta}$

$$
m l_{2}^{2} \dot{\theta} \ddot{\theta}+k l_{1}^{2} \theta \dot{\theta}+m g l_{2} \theta \dot{\theta}=0
$$

$$
m l_{2}^{2} \ddot{\theta}+k l_{1}^{2} \theta+m g l_{2} \theta=0
$$

$$
\boxed{m l_{2}^{2} \ddot{\theta}+\left(k l_{1}^{2}+m g l_{2}\right) \theta=0}
$$

$$
\boxed{\omega_{n}=\sqrt{\frac{k_{1 }l_{1}^{2}+m g l_{2}}{m l_{2}^{2}}}}
$$