Using **Euler's Relation** (Appendix A):

$$
e^{jt}=\cos{t}+j\sin{t}\qquad e^{-jt}=\cos{t}-j\sin{t}
$$

Manipulating these equations:

$$
\begin{aligned}
    \cos{t} &= \frac{1}{2}\left( e^{jt}+e^{-jt} \right)\\
    \sin{t} &= \frac{-j}{2}\left(e^{jt}-e^{-jt}\right)\\
    \text{Where:}\\
    j &= \sqrt{-1}
\end{aligned}
$$

Rewriting equation A (by math-jistu)

$$
x(t) = A\sin{\left( \omega_n t+\phi \right)}\\
$$

Where $A$ & $\phi$ are real-valued constants.

3 ways to represent harmonic motion\\
the solution for $m \ddot{x}+k x=0$

1.
$$
x(t)=a_{1} e^{j \omega_{n} t}+a_{2} e^{-j \omega_{n} t}
$$

where $a_{1}$ & $a_{2}$ are complex-valued constants

2.
$$
x(t)=A \sin \left(\omega_{n} t+\phi\right)
$$

where $A$ & $\phi$ are real valued constants

3.
$$
x(t)=A_{1} \sin \left(\omega_{n} t\right)+A_{2} \cos \left(\omega_{n}t\right)
$$

Where $A_{1}$ & $A_{2}$ are real-valued constants

***

$$
\begin{aligned}
A&=\sqrt{A_{1}^{2}+A_{2}^{2}} \\
\phi&=\tan ^{-1}\left(\frac{A_{2}}{A_{1}}\right)
A_{1}&=\left(a_{1}-a_{2}\right) j \\
A_{2}&= a_{1}+a_{2} \\
a_{1} &=\frac{A_{2}-A_{1}j}{2} \\
a_{2} &=\frac{A_{2}+A_{1}j}{2}
\end{aligned}
$$

<!-- ![](!imgdir/5b19f56b7f5a639ce7eb1c4133eda8dfef305b91.jpg) -->

# Example 1

From Handout Pg. 1

![](!imgdir/94f87eb4f86f33af5970639a21809dad2caa020c.jpg)

![](!imgdir/2c6994b9acac5ffce3cb6f0222fe2e48dfc8e39a.jpg)

# Example 1.2.1

![](!imgdir/7f6b333ce8f80abfa157b945b07d3b75f2d2333d.jpg)

![](!imgdir/9936114c88a48c0c447e253f6d16d9fac1b36d85.jpg)

# Example 1.2.2

![](!imgdir/cc0aaa551a44e71c6970ed66fb2e04390436a111.jpg)

![](!imgdir/5e3a9b5106ce491d8bd18b23645052b1a6066d1a.jpg)

# Example 1.2.3

![](!imgdir/7a4ad853783ac1d900259a081dcab8f6d0ae50cd.jpg)

![](!imgdir/bb66a8d53b382f38ca1422970fa0b4a9551f5edd.jpg)

***

![](!imgdir/309562b287750b7e461e49c481c1b60231b64381.jpg)

![](!imgdir/2a7c638c42dc375b1c3405de23f3c09b71b10dd3.jpg)
