# Problem Statement

LaGrange's formulation can also be used for non-conservative systems by adding the applied non-conservative term to the right side of the equation to get

$$
\frac{d}{d t}\left(\frac{\partial T}{\partial \dot{q}_{i}}\right)-\frac{\partial T}{\partial q_{i}}+\frac{\partial U}{\partial q_{i}}+\frac{\partial R_{i}}{\partial \dot{q}_{i}}=0
$$

Here $R_{i}$ is the Rayleigh dissipation function defined in the case of a viscous damper attached to ground by

$$
R_{i}=1 / 2\left(c \dot{q}_{i}^{2}\right)
$$

Use this extended LaGrange formation to derive the equation of motion of the damped automobile suspension driven by a dynamometer illustrated in Fig. 2. Assume here that the dynamometer drives the system such that $x=r \theta$.

![](!imgdir/screenshot_es8XRS2ryR0aqmSo.png)

# Solution

## Goal

Find EoM of damped suspension.

## Given

$$
\frac{d}{d t}\left(\frac{\partial T}{\partial \dot{q}_{i}}\right)-\frac{\partial T}{\partial q_{i}}+\frac{\partial U}{\partial q_{i}}+\frac{\partial R_{i}}{\partial \dot{q}_{i}}=0
$$

$$
R_{i}=\frac{1}{2}\left(c \dot{q}_{i}^{2}\right)
$$

$$
x=r \theta
$$

## Working

<!-- SOS -->

We can calculate:

$$
\begin{aligned}
    \frac{\partial R_{x}}{\partial \dot{x}} &= \frac{\partial}{\partial \dot{x}} \frac{1}{2}\left(c \dot{x}^{2}\right)\\
    &= c\dot{x}
\end{aligned}
$$

We can also say the following:

$$
\dot{x} = r \dot{\theta}
$$

Potential energy:

$$
\begin{aligned}
    U &= \frac{1}{2} kx^2\\
    \frac{\partial U}{\partial x} &= kx
\end{aligned}
$$

Kinetic Energy:

$$
\begin{aligned}
    T &= \frac{1}{2} m \dot{x}^2 + \frac{1}{2} J \dot{\theta}^2\\
    &= \frac{1}{2} m \dot{x}^2 + \frac{1}{2} J \left( \frac{\dot{x}}{r} \right)^2\\
    &= \frac{1}{2} m \dot{x}^2 + \frac{1}{2} J \frac{\dot{x}^2}{r^2}\\
    &= \frac{1}{2} \dot{x}^2 \left( m + \frac{J}{r^2} \right)\\
    \frac{\partial T}{\partial x} &= 0\\
    \frac{\partial T}{\partial \dot{x}} &= \dot{x} \left( m + \frac{J}{r^2} \right)\\
    \frac{d}{d t}\left(\frac{\partial T}{\partial \dot{x}}\right) &= \ddot{x} \left( m + \frac{J}{r^2} \right)\\
\end{aligned}
$$

Together, this becomes:

$$
\begin{aligned}
    \ddot{x} \left( m + \frac{J}{r^2} \right) - 0 + kx + c\dot{x} &= 0\\
    !Answer(\ddot{x} \left( m + \frac{J}{r^2} \right)+ c\dot{x} + kx)(=)(0)
\end{aligned}
$$