Consider a large plate of thickness $L$ and thermal conductivity $k$ in
which heat is generated uniformly at a rate of $\dot{e}_{\mathrm{gen}}$.
One side of the plate is insulated while the other side is exposed to an
environment at $T_{\infty}$ with a heat transfer coefficient of $h$

a.  Express the differential equation and the boundary conditions for
    steady one-dimensional heat conduction through the plate
b.  determine the variation of temperature in the plate, and
c.  obtain relations for the temperatures on both surfaces and the
    maximum temperature rise in the plate in terms of given parameters.

![](!imgdir/41e60d228a3ca828dd0919b928d6ff510fec0d73.png)

```{=tex}
\newpage
```
# Solution

## Assumptions

-   one-dimensional heat transfer
-   constant thermal conductivity

## Working

### A

From the cartesian heat diffusion equation:

$$
\frac{\partial}{\partial x}\left(k \frac{\partial T}{\partial x}\right)+\frac{\partial}{\partial y}\left(k \frac{\partial T}{\partial y}\right)+\frac{\partial}{\partial z}\left(k \frac{\partial T}{\partial z}\right)+\dot{e}_{g}=\rho c_{p} \frac{\partial T}{\partial t}
$$

we can simplify as follows:

$$
\begin{aligned}
\frac{\partial}{\partial x}\left(k \frac{\partial T}{\partial x}\right)
+
\cancelto{0}{
\frac{\partial}{\partial y}\left(k \frac{\partial T}{\partial y}\right)
}
+
\cancelto{0}{
\frac{\partial}{\partial z}\left(k \frac{\partial T}{\partial z}\right)
}
+
\dot{e}_{g}
&=
\cancelto{0}{
\rho c_{p} \frac{\partial T}{\partial t}
}\\
\frac{\partial}{\partial x}\left(k \frac{\partial T}{\partial x}\right)
+
\dot{e}_{g}
&=
0\\
\frac{\partial^2 T}{\partial x^2} + \frac{\dot{e}_g}{k} = 0\\
\end{aligned}
$$

We know also:

$$
\frac{\partial T(0)}{\partial x}=0
$$

Finally, the heat flux due to conduction and convection are equal at
$x=L$:

$$
\begin{aligned}
\dot{Q}_{\text {cond}}&=-k A_{c} \frac{d T}{d x}\\
\dot{Q}_{\text {conv}}&=h A_{s}\left(T(L)-T_{\infty}\right)\\
\therefore h \cancel{A_{s}}\left(T(L)-T_{\infty}\right) &= -k \cancel{A_{c}} \frac{d T}{d x}\\
h \left(T(L)-T_{\infty}\right) &= -k \frac{d T(L)}{d x}
\end{aligned}
$$

Thus the final equations are:

$$
\boxed{
\begin{aligned}
h \left(T(L)-T_{\infty}\right) &= -k \frac{d T(L)}{d x}\\
\frac{\partial T(0)}{\partial x}&=0\\
\frac{\partial^2 T(x)}{\partial x^2} + \frac{\dot{e}_g}{k} &= 0
\end{aligned}
}
$$

### B

We can integrate the differential equation as before:

$$
\begin{aligned}
\frac{\partial^2 T(x)}{\partial x^2} + \frac{\dot{e}_g}{k} &= 0\\
\frac{\partial^2 T(x)}{\partial x^2} &= - \frac{\dot{e}_g}{k}  \\
\int \frac{\partial^2 T(x)}{\partial x^2} dx = \frac{\partial T(x)}{\partial x} &= - x \frac{\dot{e}_g}{k} + C_1\\
\int \frac{\partial T(x)}{\partial x} dx = T(x) &= - x^2 \frac{\dot{e}_g}{2k} + x\cdot C_1 + C_2\\
\end{aligned}
$$

We can find $C_1$ by substituting the first integral:

$$
\begin{aligned}
0 &= - 0 \cdot \frac{\dot{e}_g}{k} + C_1\\
0 &= C_1
\end{aligned}
$$

Therefore:

$$
T(x) = - x^2 \frac{\dot{e}_g}{2k} + C_2
$$

and

$$
\frac{\partial T(x)}{\partial x} = - x \frac{\dot{e}_g}{k}
$$

We can find $C_2$ by substituting into the boundary condition between
conduction and convection:

$$
\begin{aligned}
h \left(T(L)-T_{\infty}\right) &= -k \frac{d T(L)}{d x}\\
h \left(- L^2 \frac{\dot{e}_g}{2k} + C_2-T_{\infty}\right) &= k L \frac{\dot{e}_g}{k}\\
-L^2 \frac{\dot{e}_g}{2k}+C_2-T_\infty &= \frac{L\dot{e}_g}{h}\\
C_2 &= T_\infty + \frac{\dot{e}_g \cdot L^2}{2k} + \frac{\dot{e}_g \cdot L}{h}
\end{aligned}
$$

Substituting into $T(x)$:

$$
\begin{aligned}
T(x) &= - x^2 \frac{\dot{e}_g}{2k} + T_\infty + \frac{\dot{e}_g \cdot L^2}{2k} + \frac{\dot{e}_g \cdot L}{h}\\
\Aboxed{T(x)&=\left( L^2 -x^2 \right) \cdot \frac{\dot{e}_g}{2k} + \frac{\dot{e}_g \cdot L}{h} + T_\infty}
\end{aligned}
$$

### C

The temperature at $x=L$ (exposed surface) is:

$$
\begin{aligned}
T(L) &= \left( L^2 -L^2 \right) \cdot \frac{\dot{e}_g}{2k} + \frac{\dot{e}_g \cdot L}{h} + T_\infty\\
\Aboxed{T(L)&=\frac{\dot{e}_g \cdot L}{h} + T_\infty}\\
\end{aligned}
$$

The temperature at $x=0$ (insulated surface) is:

$$
\begin{aligned}
T(0)&=\left( L^2 -0^2 \right) \cdot \frac{\dot{e}_g}{2k} + \frac{\dot{e}_g \cdot L}{h} + T_\infty\\
\Aboxed{T(0)&=L^2 \cdot \frac{\dot{e}_g}{2k} + \frac{\dot{e}_g \cdot L}{h} + T_\infty}\\
\end{aligned}
$$

The temperature difference is as follows:

$$
\begin{aligned}
\Delta T &= {L^2 \cdot \frac{\dot{e}_g}{2k} + \frac{\dot{e}_g \cdot L}{h} + T_\infty} - \frac{\dot{e}_g \cdot L}{h} - T_\infty\\
\Aboxed{\Delta T&=\frac{\dot{e}_g\cdot L^2}{2k}}
\end{aligned}
$$
